\begin{enumerate}
  \item \(\displaystyle \sum_{i=1}^{n} F_i \;=\; F_{n+2}-1.\)

  \item \(\displaystyle \sum_{i=1}^{n} F_{2i-1} \;=\; F_{2n}.\)

  \item \(\displaystyle \sum_{i=1}^{n} F_{2i} \;=\; F_{2n+1}-1.\)

  \item \(\displaystyle \sum_{i=1}^{n} F_i^{2} \;=\; F_n\,F_{n+1}.\)

  \item \(\displaystyle F_{n+m} \;=\; F_{n+1}F_m \;+\; F_nF_{m-1}.\)

  \item \(\displaystyle F_{n-1}F_{n+1}-F_n^{2} \;=\; (-1)^{n}.\) \hfill（Cassini 恒等式）

  \item \(\displaystyle F_{2n-1} \;=\; F_{n}^{2}+F_{n-1}^{2}.\)

  \item \(\displaystyle F_{n} \;=\; \frac{F_{n+2}+F_{n-2}}{3}.\)

  \item \(\displaystyle F_{2n} \;=\; F_n\bigl(F_{n+1}+F_{n-1}\bigr).\)

  \item 对任意 \(k\in\mathbb{N}\)，有 \(\;F_n \mid F_{nk}\).

  \item 若 \(F_a \mid F_b\)，则 \(a\mid b\).

  \item \(\displaystyle \gcd(F_n,F_m) \;=\; F_{\gcd(n,m)}.\)

  \item \(\displaystyle F_n = \frac{1}{\sqrt{5}} \left[ \left( \frac{1+\sqrt{5}}{2} \right)^n - \left( \frac{1-\sqrt{5}}{2} \right)^n \right].\)
\end{enumerate}
