\textbf{性质1：}\\[8pt]
{\large $\mathrm{C}_{\mathrm{n}}^{\mathrm{m}} = \mathrm{C}_{\mathrm{n}}^{\mathrm{n} - \mathrm{m}}$}\\[12pt]
\textbf{性质2：}\\[8pt]
{\large $\mathrm{C}_{\mathrm{n} + \mathrm{m} + 1}^{\mathrm{m}} = \sum_{i = 0}^{\mathrm{m}} \mathrm{C}_{\mathrm{n} + i}^{i}$}\\[12pt]
\textbf{性质3：}\\[8pt]
{\large $\mathrm{C}_{\mathrm{n}}^{\mathrm{m}} \cdot \mathrm{C}_{\mathrm{m}}^{\mathrm{r}} = \mathrm{C}_{\mathrm{n}}^{\mathrm{r}} \cdot \mathrm{C}_{\mathrm{n} - \mathrm{r}}^{\mathrm{m} - \mathrm{r}}$}\\[12pt]
\textbf{性质4（二项式定理）：}\\[8pt]
{\large $\sum_{i = 0}^{\mathrm{n}} \left( \mathrm{C}_{\mathrm{n}}^{i} \cdot x^{i} \right) = (1 + x)^{\mathrm{n}}$}\\[12pt]
{\large $\sum_{i = 0}^{\mathrm{n}} \mathrm{C}_{\mathrm{n}}^{i} = 2^{\mathrm{n}}$}\\[12pt]
\textbf{性质5：}\\[8pt]
{\large $\sum_{i = 0}^{\mathrm{n}} \left( (-1)^{i} \cdot \mathrm{C}_{\mathrm{n}}^{i} \right) = 0$}\\[12pt]
\textbf{性质6：}\\[8pt]
{\large $\mathrm{C}_{\mathrm{n}}^{0} + \mathrm{C}_{\mathrm{n}}^{2} + \cdots = \mathrm{C}_{\mathrm{n}}^{1} + \mathrm{C}_{\mathrm{n}}^{3} + \cdots = 2^{\mathrm{n} - 1}$}\\[12pt]
\textbf{性质7：}\\[8pt]
{\large $\mathrm{C}_{\mathrm{n} + \mathrm{m}}^{\mathrm{r}} = \sum_{i = 0}^{\min(\mathrm{n}, \mathrm{m}, \mathrm{r})} \left( \mathrm{C}_{\mathrm{n}}^{i} \cdot \mathrm{C}_{\mathrm{m}}^{\mathrm{r} - i} \right)$}\\[12pt]
{\large $\mathrm{C}_{\mathrm{n} + \mathrm{m}}^{\mathrm{n}} = \mathrm{C}_{\mathrm{n} + \mathrm{m}}^{\mathrm{m}} = \sum_{i = 0}^{\min(\mathrm{n}, \mathrm{m})} \left( \mathrm{C}_{\mathrm{n}}^{i} \cdot \mathrm{C}_{\mathrm{m}}^{i} \right), \quad (\mathrm{r} = \mathrm{n}\ |\ \mathrm{r} = \mathrm{m})$}\\[12pt]
\textbf{性质8：}\\[8pt]
{\large $\mathrm{m} \cdot \mathrm{C}_{\mathrm{n}}^{\mathrm{m}} = \mathrm{n} \cdot \mathrm{C}_{\mathrm{n} - 1}^{\mathrm{m} - 1}$}\\[12pt]
\textbf{性质9：}\\[8pt]
{\large $\sum_{i = 0}^{\mathrm{n}} \left( \mathrm{C}_{\mathrm{n}}^{i} \cdot i^2 \right) = \mathrm{n}(\mathrm{n} + 1) \cdot 2^{\mathrm{n} - 2}$}\\[12pt]
\textbf{性质10：}\\[8pt]
{\large $\sum_{i = 0}^{\mathrm{n}} \left( \mathrm{C}_{\mathrm{n}}^{i} \right)^2 = \mathrm{C}_{2\mathrm{n}}^{\mathrm{n}}$}\\[12pt]